use inttype for matrices

specs/Spec.Frodo.fst
@@ -10,9 +10,9 @@ open FStar.Math.Lemmas
 open Spec.PQ.Lib
 open Spec.Keccak
 
-assume val zqmatrix_eq:
-  #q:size_pos -> #n1:size_pos -> #n2:size_pos ->
-  a:zqmatrix_t q n1 n2 -> b:zqmatrix_t q n1 n2 -> Tot bool
+assume val matrix_eq:
+  #t:numeric_t -> #n1:size_nat -> #n2:size_nat ->
+  a:matrix_t t n1 n2 -> b:matrix_t t n1 n2 -> Tot bool
 
 assume val lbytes_eq:
   #len:size_nat -> a:lbytes len -> b:lbytes len -> Tot bool
@@ -38,24 +38,24 @@ let cshake256_frodo input_len input cstm output_len =
   squeeze s 136 output_len
 
 //FrodoKEM-640
-let params_n:size_pos = 640
-let params_logq:size_pos = 15
-let params_extracted_bits:size_pos = 2
-let crypto_bytes:size_pos = 16
+let params_n:size_nat = 640
+let params_logq:size_nat = 15
+let params_extracted_bits:size_nat = 2
+let crypto_bytes:size_nat = 16
 let cshake_frodo = cshake128_frodo
-let cdf_table_len:size_pos = 12
+let cdf_table_len:size_nat = 12
 let cdf_table : lseq size_nat cdf_table_len =
   let cdf_table0: list size_nat = [4727; 13584; 20864; 26113; 29434; 31278; 32176; 32560; 32704; 32751; 32764; 32767] in
   assert_norm (List.Tot.length cdf_table0 = cdf_table_len);
   createL cdf_table0
 
-let bytes_seed_a:size_pos = 16
-let params_nbar:size_pos = 8
-let params_q:size_pos = pow2 params_logq
-let bytes_mu:size_pos = (params_extracted_bits * params_nbar * params_nbar) / 8
-let crypto_publickeybytes:size_pos  = bytes_seed_a + (params_logq * params_n * params_nbar) / 8
-let crypto_secretkeybytes:size_pos  = crypto_bytes + crypto_publickeybytes
-let crypto_ciphertextbytes:size_pos = ((params_nbar * params_n + params_nbar * params_nbar) * params_logq) / 8 + crypto_bytes
+let bytes_seed_a:size_nat = 16
+let params_nbar:size_nat = 8
+let params_q:size_nat = pow2 params_logq
+let bytes_mu:size_nat = (params_extracted_bits * params_nbar * params_nbar) / 8
+let crypto_publickeybytes:size_nat  = bytes_seed_a + (params_logq * params_n * params_nbar) / 8
+let crypto_secretkeybytes:size_nat  = crypto_bytes + crypto_publickeybytes
+let crypto_ciphertextbytes:size_nat = ((params_nbar * params_n + params_nbar * params_nbar) * params_logq) / 8 + crypto_bytes
 
 val ec:k:size_nat{k < pow2 params_extracted_bits} -> Tot (r:size_nat{r < pow2 params_logq})
 let ec k = k * pow2 (params_logq - params_extracted_bits)
@@ -84,31 +84,33 @@ let lemma_dc_ec k =
   small_division_lemma_1 1 (pow2 1);
   small_modulo_lemma_1 k (pow2 params_extracted_bits)
 
+unfold type elem_t:numeric_t = NATm params_q
+
 assume val frodo_key_encode:
   b:size_nat{(params_nbar * params_nbar * b) / 8 < max_size_t} ->
   a:lbytes ((params_nbar * params_nbar * b) / 8) ->
-  Tot (zqmatrix_t params_q params_nbar params_nbar)
+  Tot (matrix_t elem_t params_nbar params_nbar)
 //let frodo_key_encode b a = admit()
 
 assume val frodo_key_decode:
   b:size_nat{(params_nbar * params_nbar * b) / 8 < max_size_t} ->
-  a:zqmatrix_t params_q params_nbar params_nbar ->
+  a:matrix_t elem_t params_nbar params_nbar ->
   Tot (lbytes ((params_nbar * params_nbar * b) / 8))
 //let frodo_key_decode b a = admit()
 
 assume val frodo_pack:
-  n1:size_pos -> n2:size_pos ->
-  a:zqmatrix_t params_q n1 n2 ->
+  n1:size_nat -> n2:size_nat ->
+  a:matrix_t elem_t n1 n2 ->
   d:size_nat{(d * n1 * n2) / 8 < max_size_t} -> Tot (lbytes ((d * n1 * n2) / 8))
 //let frodo_pack n1 n2 a d =
 
 assume val frodo_unpack:
-  n1:size_pos -> n2:size_pos ->
+  n1:size_nat -> n2:size_nat ->
   d:size_nat{(d * n1 * n2) / 8 < max_size_t} -> b:lbytes ((d * n1 * n2) / 8) ->
-  Tot (zqmatrix_t params_q n1 n2)
+  Tot (matrix_t elem_t n1 n2)
 //let frodo_unpack n1 n2 d b = admit()
 
-val frodo_sample: r:uint16 -> Tot (zqelem_t params_q)
+val frodo_sample: r:uint16 -> Tot (uint_t elem_t)
 #reset-options "--z3rlimit 50 --max_fuel 1"
 let frodo_sample r =
   let t = r >>. u32 1 in
@@ -119,57 +121,56 @@ let frodo_sample r =
   (fun z e ->
     let e = if (uint_to_nat t > cdf_table.[z]) then e + 1 else e in e
   ) e in
-  assume (e < cdf_table_len);
   let e = (FStar.Math.Lib.powx (-1) (uint_to_nat r0)) * e in
-  assume (-cdf_table_len < e /\ e < cdf_table_len);
-  zqelem (e + params_q)
+  numeric (e % modulus elem_t)
 
 val frodo_sample_matrix:
-  n1:size_pos -> n2:size_pos{2 * n1 * n2 < max_size_t} ->
+  n1:size_nat -> n2:size_nat{2 * n1 * n2 < max_size_t} ->
   seedLen:size_nat -> seed:lbytes seedLen ->
-  ctr:uint16 -> Tot (zqmatrix_t params_q n1 n2)
+  ctr:uint16 -> Tot (matrix_t elem_t n1 n2)
 let frodo_sample_matrix n1 n2 seedLen seed ctr =
   let r = cshake_frodo seedLen seed ctr (2 * n1 * n2) in
-  let res = zqmatrix_create params_q n1 n2 in
+  let res = matrix_create elem_t n1 n2 in
   repeati n1
   (fun i res ->
     repeati n2
     (fun j res ->
       assume (2 * (n2 * i + j) + 2 <= 2 * n1 * n2);
       let res_ij = sub r (2 * (n2 * i + j)) 2 in
-      set res i j (frodo_sample (uint_from_bytes_le #U16 res_ij))
+      mset res i j (frodo_sample (uint_from_bytes_le #U16 res_ij))
     ) res
   ) res
 
 val frodo_sample_matrix_tr:
-  n1:size_pos -> n2:size_pos{2 * n1 * n2 < max_size_t} ->
+  n1:size_nat -> n2:size_nat{2 * n1 * n2 < max_size_t} ->
   seedLen:size_nat -> seed:lbytes seedLen ->
-  ctr:uint16 -> Tot (zqmatrix_t params_q n1 n2)
+  ctr:uint16 -> Tot (matrix_t elem_t n1 n2)
 let frodo_sample_matrix_tr n1 n2 seedLen seed ctr =
   let r = cshake_frodo seedLen seed ctr (2 * n1 * n2) in
-  let res = zqmatrix_create params_q n1 n2 in
+  let res = matrix_create elem_t n1 n2 in
   repeati n1
   (fun i res ->
     repeati n2
     (fun j res ->
       assume (2 * (n1 * j + i) + 2 <= 2 * n1 * n2);
       let res_ij = sub r (2 * (n1 * j + i)) 2 in
-      set res i j (frodo_sample (uint_from_bytes_le #U16 res_ij))
+      mset res i j (frodo_sample (uint_from_bytes_le #U16 res_ij))
     ) res
   ) res
 
 val frodo_gen_matrix_cshake:
-  n:size_pos{2 * n < max_size_t /\ 256 + n < maxint U16} -> seedLen:size_nat -> seed:lbytes seedLen ->
-  Tot (zqmatrix_t params_q n n)
+  n:size_nat{2 * n < max_size_t /\ 256 + n < maxint U16} ->
+  seedLen:size_nat -> seed:lbytes seedLen ->
+  Tot (matrix_t elem_t n n)
 let frodo_gen_matrix_cshake n seedLen seed =
-  let res = zqmatrix_create params_q n n in
+  let res = matrix_create elem_t n n in
   repeati n
   (fun i res ->
     let res_i = cshake128_frodo seedLen seed (u16 (256 + i)) (2 * n) in
     repeati n
     (fun j res ->
       let res_ij = uint_from_bytes_le #U16 (sub res_i (j * 2) 2) in
-      set res i j (zqelem #params_q (uint_to_nat res_ij))
+      mset res i j (numeric (uint_to_nat res_ij % modulus elem_t))
     ) res
   ) res
 
@@ -177,7 +178,8 @@ let frodo_gen_matrix = frodo_gen_matrix_cshake
 
 val crypto_kem_keypair:
   coins:lbytes (2 * crypto_bytes + bytes_seed_a) ->
-  Tot (tuple2 (lbytes crypto_publickeybytes) (tuple2 (lbytes crypto_secretkeybytes) (zqmatrix_t params_q params_n params_nbar)))
+  Tot (tuple2 (lbytes crypto_publickeybytes)
+	      (tuple2 (lbytes crypto_secretkeybytes) (matrix_t elem_t params_n params_nbar)))
 let crypto_kem_keypair coins =
   let s = sub coins 0 crypto_bytes in
   let seed_e = sub coins crypto_bytes crypto_bytes in
@@ -186,12 +188,12 @@ let crypto_kem_keypair coins =
   let a_matrix = frodo_gen_matrix params_n bytes_seed_a seed_a in
   let s_matrix = frodo_sample_matrix_tr params_n params_nbar crypto_bytes seed_e (u16 1) in
   let e_matrix = frodo_sample_matrix params_n params_nbar crypto_bytes seed_e (u16 2) in
-  let b_matrix = zqmatrix_add (zqmatrix_mul a_matrix s_matrix) e_matrix in
+  let b_matrix = matrix_add (matrix_mul a_matrix s_matrix) e_matrix in
   let b = frodo_pack params_n params_nbar b_matrix params_logq in
 
   let pk = concat seed_a b in
   let sk = concat s pk in
-  (pk,  (sk, s_matrix))
+  (pk, (sk, s_matrix))
 
 val crypto_kem_enc:
   coins:lbytes bytes_mu -> pk:lbytes crypto_publickeybytes ->
@@ -208,15 +210,15 @@ let crypto_kem_enc coins pk =
   let sp_matrix = frodo_sample_matrix params_nbar params_n crypto_bytes seed_e (u16 4) in
   let ep_matrix = frodo_sample_matrix params_nbar params_n crypto_bytes seed_e (u16 5) in
   let a_matrix = frodo_gen_matrix params_n bytes_seed_a seed_a in
-  let bp_matrix = zqmatrix_add (zqmatrix_mul sp_matrix a_matrix) ep_matrix in
+  let bp_matrix = matrix_add (matrix_mul sp_matrix a_matrix) ep_matrix in
   let c1 = frodo_pack params_nbar params_n bp_matrix params_logq in
 
   let epp_matrix = frodo_sample_matrix params_nbar params_nbar crypto_bytes seed_e (u16 6) in
   let b_matrix = frodo_unpack params_n params_nbar params_logq b in
-  let v_matrix = zqmatrix_add (zqmatrix_mul sp_matrix b_matrix) epp_matrix in
+  let v_matrix = matrix_add (matrix_mul sp_matrix b_matrix) epp_matrix in
 
   let mu_encode = frodo_key_encode params_extracted_bits coins in
-  let c_matrix = zqmatrix_add v_matrix mu_encode in
+  let c_matrix = matrix_add v_matrix mu_encode in
   let c2 = frodo_pack params_nbar params_nbar c_matrix params_logq in
 
   let ss_init = concat c1 (concat c2 (concat k d)) in
@@ -227,7 +229,7 @@ let crypto_kem_enc coins pk =
 
 val crypto_kem_dec:
   ct:lbytes crypto_ciphertextbytes ->
-  sk:tuple2 (lbytes crypto_secretkeybytes) (zqmatrix_t params_q params_n params_nbar) ->
+  sk:tuple2 (lbytes crypto_secretkeybytes) (matrix_t elem_t params_n params_nbar) ->
   Tot (lbytes crypto_bytes)
 let crypto_kem_dec ct sk =
   let c1Len = (params_logq * params_nbar * params_n) / 8 in
@@ -244,7 +246,7 @@ let crypto_kem_dec ct sk =
 
   let bp_matrix = frodo_unpack params_nbar params_n params_logq c1 in
   let c_matrix = frodo_unpack params_nbar params_nbar params_logq c2 in
-  let m_matrix = zqmatrix_sub c_matrix (zqmatrix_mul bp_matrix s_matrix) in
+  let m_matrix = matrix_sub c_matrix (matrix_mul bp_matrix s_matrix) in
   let mu_decode = frodo_key_decode params_extracted_bits m_matrix in
 
   let g = cshake_frodo (crypto_publickeybytes + (params_nbar * params_nbar * params_extracted_bits) / 8) (concat pk mu_decode)  (u16 3) (3 * crypto_bytes) in
@@ -255,20 +257,20 @@ let crypto_kem_dec ct sk =
   let sp_matrix = frodo_sample_matrix params_nbar params_n crypto_bytes seed_ep (u16 4) in
   let ep_matrix = frodo_sample_matrix params_nbar params_n crypto_bytes seed_ep (u16 5) in
   let a_matrix = frodo_gen_matrix params_n bytes_seed_a seed_a in
-  let bpp_matrix = zqmatrix_add (zqmatrix_mul sp_matrix a_matrix) ep_matrix in
+  let bpp_matrix = matrix_add (matrix_mul sp_matrix a_matrix) ep_matrix in
 
   let epp_matrix = frodo_sample_matrix params_nbar params_nbar crypto_bytes seed_ep (u16 6) in
   let b_matrix = frodo_unpack params_n params_nbar params_logq b in
-  let v_matrix = zqmatrix_add (zqmatrix_mul sp_matrix b_matrix) epp_matrix in
+  let v_matrix = matrix_add (matrix_mul sp_matrix b_matrix) epp_matrix in
 
   let mu_encode = frodo_key_encode params_extracted_bits mu_decode in
-  let cp_matrix = zqmatrix_add v_matrix mu_encode in
+  let cp_matrix = matrix_add v_matrix mu_encode in
 
   let ss_init = concat c1 c2 in
   let ss_init_len = (params_logq * params_nbar * params_n) / 8 + (params_logq * params_nbar * params_nbar) / 8 + 2 * crypto_bytes in
   let ss_init1:lbytes ss_init_len = concat ss_init (concat kp d) in
   let ss_init2:lbytes ss_init_len = concat ss_init (concat s d) in
-  let bcond = (lbytes_eq #crypto_bytes d dp) && (zqmatrix_eq #params_q #params_nbar #params_n bp_matrix bpp_matrix) && (zqmatrix_eq #params_q #params_nbar #params_nbar c_matrix cp_matrix) in
+  let bcond = (lbytes_eq d dp) && (matrix_eq bp_matrix bpp_matrix) && (matrix_eq c_matrix cp_matrix) in
   let ss_init = if (bcond) then ss_init1 else ss_init2 in
   let ss = cshake_frodo ss_init_len ss_init (u16 7) crypto_bytes in
   ss
